WIP: Framework for correctness of transformations

src/coq/TopLevel.v
@@ -61,15 +61,11 @@ Module TopLevelEnv <: Environment.
   Definition memory     := M.memory_stack.
   Definition stack      := @stack (list (raw_id * uvalue)).
 
-(* Definition local_env  := FMapAList.alist raw_id uvalue. *)
-(* Definition global_env := FMapAList.alist raw_id dvalue. *)
+  Open Scope string_scope.
 
+  (* end hide *)
 
-Open Scope string_scope.
-
-(* end hide *)
-
-(**
+  (**
    This file ties things together to concretely defines the semantics of a [Vellvm]
    program. It covers two main tasks to do so: to initialize the memory, and to
    chain together the successive interpreters.
@@ -79,145 +75,138 @@ Open Scope string_scope.
    internal non-determinism due to under-defined values into the non-determinism
    monad; and an executable one, that arbitrarily interpret under-defined values
    by setting its bits to 0.
- *)
+   *)
 
-(** Initialization
+  (** Initialization
     The initialization phase allocates and initializes globals,
     and allocates function pointers.
     This initialization phase is internalized in [Vellvm], it is
     an [itree] as any other.
- *)
+   *)
 
-Definition allocate_global (g:global dtyp) : itree L0 unit :=
-  (vis (Alloca (g_typ g)) (fun v => trigger (GlobalWrite (g_ident g) v))).
+  Definition allocate_global (g:global dtyp) : itree L0 unit :=
+    (vis (Alloca (g_typ g)) (fun v => trigger (GlobalWrite (g_ident g) v))).
 
-Definition allocate_globals (gs:list (global dtyp)) : itree L0 unit :=
-  map_monad_ allocate_global gs.
+  Definition allocate_globals (gs:list (global dtyp)) : itree L0 unit :=
+    map_monad_ allocate_global gs.
 
-(* Who is in charge of allocating the addresses for external functions declared in this mcfg? *)
-Definition allocate_declaration (d:declaration dtyp) : itree L0 unit :=
-  (* SAZ TODO:  Don't allocate pointers for LLVM intrinsics declarations *)
+  (* Who is in charge of allocating the addresses for external functions declared in this mcfg? *)
+  Definition allocate_declaration (d:declaration dtyp) : itree L0 unit :=
+    (* SAZ TODO:  Don't allocate pointers for LLVM intrinsics declarations *)
     vis (Alloca DTYPE_Pointer) (fun v => trigger (GlobalWrite (dc_name d) v)).
 
-Definition allocate_declarations (ds:list (declaration dtyp)) : itree L0 unit :=
-  map_monad_ allocate_declaration ds.
+  Definition allocate_declarations (ds:list (declaration dtyp)) : itree L0 unit :=
+    map_monad_ allocate_declaration ds.
 
-Definition initialize_global (g:global dtyp) : itree exp_E unit :=
-  let dt := (g_typ g) in
-  a <- trigger (GlobalRead (g_ident g));;
-  uv <- match (g_exp g) with
-       | None => ret (UVALUE_Undef dt)
-       | Some e => D.denote_exp (Some dt) e
-       end ;;
-  (* CB TODO: Do we need pick here? *)
-  dv <- trigger (pick uv True) ;;
-  trigger (Store a dv).
+  Definition initialize_global (g:global dtyp) : itree exp_E unit :=
+    let dt := (g_typ g) in
+    a <- trigger (GlobalRead (g_ident g));;
+      uv <- match (g_exp g) with
+            | None => ret (UVALUE_Undef dt)
+            | Some e => D.denote_exp (Some dt) e
+            end ;;
+      (* CB TODO: Do we need pick here? *)
+      dv <- trigger (pick uv True) ;;
+      trigger (Store a dv).
 
-Definition initialize_globals (gs:list (global dtyp)): itree exp_E unit :=
-  map_monad_ initialize_global gs.
+  Definition initialize_globals (gs:list (global dtyp)): itree exp_E unit :=
+    map_monad_ initialize_global gs.
 
-Definition build_global_environment (CFG : CFG.mcfg dtyp) : itree L0 unit :=
-  allocate_globals (m_globals CFG) ;;
-  allocate_declarations ((m_declarations CFG) ++ (List.map (df_prototype) (m_definitions CFG)));;
-  translate _exp_E_to_L0 (initialize_globals (m_globals CFG)).
+  Definition build_global_environment (CFG : CFG.mcfg dtyp) : itree L0 unit :=
+    allocate_globals (m_globals CFG) ;;
+                     allocate_declarations ((m_declarations CFG) ++ (List.map (df_prototype) (m_definitions CFG)));;
+                     translate _exp_E_to_L0 (initialize_globals (m_globals CFG)).
 
-(** Local environment implementation
+  (** Local environment implementation
     The map-based handlers are defined parameterized over a domain of key and value.
     We now pick concrete such domain.
     Note that while local environments may store under-defined values,
     global environments are statically guaranteed to store [dvalue]s.
- *)
-Definition function_env := FMapAList.alist dvalue D.function_denotation.
+   *)
+  Definition function_env := FMapAList.alist dvalue D.function_denotation.
 
-(**
+  (**
    Denotes a function and returns its pointer.
- *)
+   *)
 
-Definition address_one_function (df : definition dtyp (CFG.cfg dtyp)) : itree L0 (dvalue * D.function_denotation) :=
-  let fid := (dc_name (df_prototype df)) in
-  fv <- trigger (GlobalRead fid) ;;
-  ret (fv, D.denote_function df).
+  Definition address_one_function (df : definition dtyp (CFG.cfg dtyp)) : itree L0 (dvalue * D.function_denotation) :=
+    let fid := (dc_name (df_prototype df)) in
+    fv <- trigger (GlobalRead fid) ;;
+       ret (fv, D.denote_function df).
 
-(* (for now) assume that [main (i64 argc, i8** argv)]
+  (* (for now) assume that [main (i64 argc, i8** argv)]
     pass in 0 and null as the arguments to main
     Note: this isn't compliant with standard C semantics
-*)
-Definition main_args := [DV.DVALUE_I64 (DynamicValues.Int64.zero);
-                         DV.DVALUE_Addr (Memory.A.null)
-                        ].
+   *)
+  Definition main_args := [DV.DVALUE_I64 (DynamicValues.Int64.zero);
+                             DV.DVALUE_Addr (Memory.A.null)
+                          ].
 
-(**
+  (**
    Transformation and normalization of types.
-*)
-Definition eval_typ (CFG:CFG.mcfg typ) (t:typ) : dtyp :=
-      TypeUtil.normalize_type_dtyp (m_type_defs CFG) t.
+   *)
+  Definition eval_typ (CFG:CFG.mcfg typ) (t:typ) : dtyp :=
+    TypeUtil.normalize_type_dtyp (m_type_defs CFG) t.
 
-Definition normalize_types (CFG:(CFG.mcfg typ)) : (CFG.mcfg dtyp) :=
-  TransformTypes.fmap_mcfg _ _ (eval_typ CFG) CFG.
+  Definition normalize_types (CFG:(CFG.mcfg typ)) : (CFG.mcfg dtyp) :=
+    TransformTypes.fmap_mcfg _ _ (eval_typ CFG) CFG.
 
-(**
+  (**
    We are now ready to define our semantics. Guided by the events and handlers,
    we work in layers: the first layer is defined as the uninterpreted [itree]
    resulting from the denotation of the LLVM program. Each successive handler
    then transform a tree at layer n to a tree at layer (n+1).
- *)
-(**
+   *)
+  (**
    In order to limit bloated type signature, we name the successive return types.
-*)
+   *)
 
-Notation res_L0 := uvalue (* (only parsing) *).
-Notation res_L1 := (global_env * res_L0)%type (* (only parsing) *).
-Notation res_L2 := (local_env * stack * res_L1)%type (* (only parsing) *).
-Notation res_L3 := (memory * res_L2)%type (* (only parsing) *).
-Notation res_L4 := (memory * (local_env * stack * (global_env * dvalue)))%type (* (only parsing) *).
+  Notation res_L0 := uvalue (* (only parsing) *).
+  Notation res_L1 := (global_env * res_L0)%type (* (only parsing) *).
+  Notation res_L2 := (local_env * stack * res_L1)%type (* (only parsing) *).
+  Notation res_L3 := (memory * res_L2)%type (* (only parsing) *).
+  Notation res_L4 := (memory * (local_env * stack * (global_env * dvalue)))%type (* (only parsing) *).
 
-(* Initialization and denotation of a Vellvm program *)
-Definition build_L0 (mcfg : CFG.mcfg dtyp) : itree L0 res_L0 :=
-  build_global_environment mcfg ;;
-  'defns <- map_monad address_one_function (m_definitions mcfg) ;;
-  'addr <- trigger (GlobalRead (Name "main")) ;;
-  D.denote_mcfg defns DTYPE_Void addr main_args.
+  (* Initialization and denotation of a Vellvm program *)
+  Definition build_L0 (mcfg : CFG.mcfg dtyp) : itree L0 res_L0 :=
+    build_global_environment mcfg ;;
+                             'defns <- map_monad address_one_function (m_definitions mcfg) ;;
+                             'addr <- trigger (GlobalRead (Name "main")) ;;
+                             D.denote_mcfg defns DTYPE_Void addr main_args.
 
-(* Interpretation of the global environment *)
-Definition build_L1 (trace : itree L0 res_L0) : itree L1 res_L1 :=
-             interp_global trace [].
+  (* Interpretation of the global environment *)
+  Definition build_L1 (trace : itree L0 res_L0) : itree L1 res_L1 :=
+    interp_global trace [].
 
-(* Interpretation of the local environment: map and stack *)
-Definition build_L2 (trace : itree L1 res_L1) : itree L2 res_L2 :=
-  interp_local_stack (@handle_local _ _ _ _ _ _ _) trace ([], []).
+  (* Interpretation of the local environment: map and stack *)
+  Definition build_L2 (trace : itree L1 res_L1) : itree L2 res_L2 :=
+    interp_local_stack (@handle_local _ _ _ _ _ _ _) trace ([], []).
 
-(* Interpretation of the memory *)
-Definition build_L3 (trace : itree L2 res_L2) : itree L3 res_L3 :=
-  M.interp_memory trace (M.empty, [[]]).
+  (* Interpretation of the memory *)
+  Definition build_L3 (trace : itree L2 res_L2) : itree L3 res_L3 :=
+    M.interp_memory trace (M.empty, [[]]).
 
-(* Interpretation of under-defined values as 0 *)
-(* YZ: I'm not fully convinced by this, this translate for the return value is awkward. *)
-Definition build_L4 (trace : itree L3 res_L3) : itree L4 res_L4 :=
-  '(m, (env, (genv, uv))) <- (P.interp_undef trace);;
-   dv <- translate _failure_UB_to_L4 (P.concretize_uvalue uv);;
-   ret (m, (env, (genv, dv))).
+  (* Interpretation of under-defined values as 0 *)
+  (* YZ: I'm not fully convinced by this, this translate for the return value is awkward. *)
+  Definition build_L4 (trace : itree L3 res_L3) : itree L4 res_L4 :=
+    '(m, (env, (genv, uv))) <- (P.interp_undef trace);;
+     dv <- translate _failure_UB_to_L4 (P.concretize_uvalue uv);;
+     ret (m, (env, (genv, dv))).
 
-(* Interpretation of under-defined values as 0 *)
-Definition model_L4 (trace : itree L3 res_L3) : PropT (itree L4) res_L3 :=
-  P.model_undef trace.
+  (* Interpretation of under-defined values as 0 *)
+  Definition model_L4 (trace : itree L3 res_L3) : PropT (itree L4) res_L3 :=
+    P.model_undef trace.
 
-Definition build_L5 (trace : itree L4 res_L4) : itree L5 res_L4 :=
-  interp_UB trace.
+  Definition build_L5 (trace : itree L4 res_L4) : itree L5 res_L4 :=
+    interp_UB trace.
 
-Definition model_L5 (trace : PropT (itree L4) res_L3) : PropT (itree L5) res_L3 :=
-  model_UB trace.
+  Definition model_L5 (trace : PropT (itree L4) res_L3) : PropT (itree L5) res_L3 :=
+    model_UB trace.
 
-End TopLevelEnv.
+  (** Definition of the executable interpreter *)
 
-Import TopLevelEnv.
-
-Definition interpreter_user (user_intrinsics: IS.intrinsic_definitions) (prog: list (toplevel_entity typ (list (block typ)))) : itree L5 res_L4 :=
-  let scfg := Vellvm.AstLib.modul_of_toplevel_entities _ prog in
-
-  match CFG.mcfg_of_modul _ scfg with
-  | Some ucfg =>
-
-    let mcfg := normalize_types ucfg in
+  Definition interpret_mcfg_user (user_intrinsics: IS.intrinsic_definitions) (prog: CFG.mcfg typ) : itree L5 res_L4 :=
+    let mcfg := normalize_types prog in
 
     let L0_trace          := build_L0 mcfg in
     let L0_trace'         := INT.interpret_intrinsics user_intrinsics L0_trace in
@@ -227,21 +216,24 @@ Definition interpreter_user (user_intrinsics: IS.intrinsic_definitions) (prog: l
     let L4_Trace          := build_L4 L3_Trace in
     let L5_Trace          := build_L5 L4_Trace in
     debug "Starting to interpret the program.";;
-    L5_Trace
+          L5_Trace.
 
-  | None => raise "Ill-formed program: mcfg_of_modul failed."
-  end.
+  Definition interpreter_user (user_intrinsics: IS.intrinsic_definitions) (prog: list (toplevel_entity typ (list (block typ)))) : itree L5 res_L4 :=
+    let scfg := Vellvm.AstLib.modul_of_toplevel_entities _ prog in
 
-(* Users may define their own interpreter by providing additional intrinsics *)
-Definition interpreter := interpreter_user [].
+    match CFG.mcfg_of_modul _ scfg with
+    | Some ucfg => interpret_mcfg_user user_intrinsics ucfg
 
-Definition model_user (user_intrinsics: IS.intrinsic_definitions) (prog: list (toplevel_entity typ (list (block typ)))) :
-  PropT (itree L5) res_L3 :=
-  let scfg := Vellvm.AstLib.modul_of_toplevel_entities _ prog in
+    | None => raise "Ill-formed program: mcfg_of_modul failed."
+    end.
 
-  match  CFG.mcfg_of_modul _ scfg with
-  | Some ucfg =>
-    let mcfg := normalize_types ucfg in
+  (* Users may define their own interpreter by providing additional intrinsics *)
+  Definition interpreter := interpreter_user [].
+
+  (** Definition of the semantics -- a propositional model that serves as official specification of the language *)
+
+  Definition model_mcfg_user (user_intrinsics: IS.intrinsic_definitions) (prog: CFG.mcfg typ) : PropT (itree L5) res_L3 :=
+    let mcfg := normalize_types prog in
 
     let L0_trace        := build_L0 mcfg in
     let L0_trace'       := INT.interpret_intrinsics user_intrinsics L0_trace in
@@ -250,11 +242,20 @@ Definition model_user (user_intrinsics: IS.intrinsic_definitions) (prog: list (t
     let L3_trace        := build_L3 L2_trace in
     let L4_trace        := model_L4 L3_trace in
     let L5_trace        := model_L5 L4_trace in
-    L5_trace
+    L5_trace.
 
-  | None => lift (raise "Ill-formed program: mcfg_of_modul failed.")
-  end.
+  Definition model_user (user_intrinsics: IS.intrinsic_definitions) (prog: list (toplevel_entity typ (list (block typ)))) :
+    PropT (itree L5) res_L3 :=
+    let scfg := Vellvm.AstLib.modul_of_toplevel_entities _ prog in
 
-(* Users may define their own model by providing additional intrinsics *)
-Definition model := model_user [].
+    match  CFG.mcfg_of_modul _ scfg with
+    | Some ucfg => model_mcfg_user user_intrinsics ucfg
 
+    | None => lift (raise "Ill-formed program: mcfg_of_modul failed.")
+    end.
+
+  (* Users may define their own model by providing additional intrinsics *)
+  Definition model_mcfg := model_mcfg_user [].
+  Definition model := model_user [].
+
+End TopLevelEnv.
