src/coq/TopLevelRefinements.v
@@ -7,6 +7,7 @@ From ITree Require Import
      Eq.Eq.
 
 From Vellvm Require Import
+     CFG
      Memory
      Refinement
      Environment
@@ -15,29 +16,38 @@ From Vellvm Require Import
      Handlers.Stack.
 
 From ExtLib Require Import
-     Structures.Functor
-     
-.
+     Structures.Functor.
 
 From Coq Require Import
      Logic
-     Morphisms.
+     Morphisms
+     Relations.
 
 Import ITree.Basics.Basics.Monads.
-Require Import Relations.
 
 Module R := Refinement.Make(Memory.A)(IO)(TopLevelEnv).
 Import R.
 Import TopLevelEnv.
 
-Require Import Omega.
+(** The module _Refinement.Make_ defines a series of refinements between
+    [itree]s at the various signatures of events a Vellvm goes through during
+    the chain of interpretations leading to the definition of the model.
+    These refinements state set inclusion of the concretization of the
+    returned under-defined values, but impose no constraints on the states.
 
-(* CB: Does this already exist? *)
-Lemma subrelation_R_TT: 
+    In this module, we show that these refinements define a chain of growing
+    relations when composed with the bits of interpretations relating each
+    level.
+
+    Finally, this allows us to lift these relations on [itree]s to a growing
+    chain of relations on [mcfg typ].
+ *)
+
+(** BEGIN TO MOVE *)
+Lemma subrelation_R_TT:
   forall A (R : relation A), subrelation R TT.
 Proof. firstorder. Qed.
 
-(* CB: Does this already exist? *)
 Lemma subrelation_prod_left :
   forall A B (R R' : relation A) (R2 : relation B), subrelation R R' -> subrelation (R × R2) (R' × R2).
 Proof.
@@ -52,42 +62,160 @@ Lemma eutt_tt_to_eq_prod :
     eutt (eq × RR) t1 t2 -> eutt (TT × RR) t1 t2.
 Proof.
   intros X R RR E t1 t2 Heutt.
-
   unfold eutt.
-  About eqit_mon.
   apply (eqit_mon (eq × RR) (TT × RR) true true true true); trivial.
   intros x0 x1 PR.
   eapply subrelation_prod_left. apply subrelation_R_TT. all: apply PR.
 Qed.
 
+(* Instance interp_prop_Proper : *)
+(*   forall R E F G (t : itree (E +' G) R) (RR : relation R) (h : (E +' F +' G) ~> PropT.PropT (itree (E +' G))), *)
+(*     Proper (@eutt (E +' F +' G) _ _ RR ==> iff) (fun t' => @PropT.interp_prop (E +' F +' G) _ _ _ _ h _ t' t). *)
+(* Proof. *)
+(*   intros R E F G t RR h. *)
+(*   intros t1 t2 Heutt. *)
+(*   unfold PropT.PropT in h. unfold Ensembles.Ensemble in h. *)
+(* Admitted. *)
+
+(* This formulation should be easier to use *)
+Instance interp_prop_Proper :
+  forall R E F G (RR : relation R) (h : (E +' F +' G) ~> PropT.PropT (itree (E +' G))),
+    Proper (@eutt (E +' F +' G) _ _ RR ==> eq ==> Basics.impl) (@PropT.interp_prop (E +' F +' G) _ _ _ _ h R).
+Proof.
+  intros R E F G t RR h.
+  intros t1 t2 Heutt.
+  unfold PropT.PropT in h. unfold Ensembles.Ensemble in h.
+Admitted.
+
+Hint Unfold TT.
+Instance TT_equiv :
+  forall A, Equivalence (@TT A).
+Proof.
+  intros A; split; repeat intro; auto.
+Qed.
+
+(** END TO MOVE *)
+
+
+(** We first prove that the [itree] refinement at level [i] entails the
+    refinement at level [i+1] after running the [i+1] level of interpretation
+ *)
+
 Lemma refine_01: forall t1 t2,
     refine_L0 t1 t2 -> refine_L1 (build_L1 t1) (build_L1 t2).
 Proof.
   intros t1 t2 H.
-
-  unfold refine_L1. unfold eutt.
-  unfold refine_res1.
-
-  apply eutt_tt_to_eq_prod.
-  apply eutt_interp_state_gen; auto.
+  apply eutt_tt_to_eq_prod, eutt_interp_state_gen; auto.
 Qed.
 
 Lemma refine_12 : forall t1 t2,
     refine_L1 t1 t2 -> refine_L2 (build_L2 t1) (build_L2 t2).
 Proof.
   intros t1 t2 H.
-  apply eutt_tt_to_eq_prod.
-  apply eutt_interp_state_gen; auto.
+  apply eutt_tt_to_eq_prod, eutt_interp_state_gen; auto.
 Qed.
 
 Lemma refine_23 : forall t1 t2,
     refine_L2 t1 t2 -> refine_L3 (build_L3 t1) (build_L3 t2).
 Proof.
   intros t1 t2 H.
-  apply eutt_tt_to_eq_prod.
-  apply eutt_interp_state_gen; auto.
+  apply eutt_tt_to_eq_prod, eutt_interp_state_gen; auto.
 Qed.
 
+(* Things are different for L4 and L5: we get into the [Prop] monad. *)
+Lemma refine_34 : forall t1 t2,
+    refine_L3 t1 t2 -> refine_L4 (model_L4 t1) (model_L4 t2).
+Proof.
+  intros t1 t2 H t Ht.
+  exists t; split.
+  - unfold model_L4, P.model_undef in *.
+    unfold IO.L3 in *.
+    match goal with |- PropT.interp_prop ?x _ _ _ => remember x as h end.
+    eapply interp_prop_Proper; eauto.
+  - reflexivity.
+Qed.
+
+Lemma refine_45 : forall t1 t2,
+    refine_L4 t1 t2 -> refine_L5 (model_L5 t1) (model_L5 t2).
+Proof.
+Admitted.
+
+(**
+   We now define partial interpretations in order to define refinements of [mcfg]s
+ *)
+
+Definition build_to_L1 user_intrinsics (prog: mcfg typ) :=
+  let mcfg := normalize_types prog in
+  let L0_trace        := build_L0 mcfg in
+  let L0_trace'       := INT.interpret_intrinsics user_intrinsics L0_trace in
+  let L1_trace        := build_L1 L0_trace' in
+  L1_trace.
+
+Definition build_to_L2 user_intrinsics (prog: mcfg typ) :=
+  let mcfg := normalize_types prog in
+  let L0_trace        := build_L0 mcfg in
+  let L0_trace'       := INT.interpret_intrinsics user_intrinsics L0_trace in
+  let L1_trace        := build_L1 L0_trace' in
+  let L2_trace        := build_L2 L1_trace in
+  L2_trace.
+
+Definition build_to_L3 (user_intrinsics: IS.intrinsic_definitions) (prog: mcfg typ) :=
+  let mcfg := normalize_types prog in
+
+  let L0_trace        := build_L0 mcfg in
+  let L0_trace'       := INT.interpret_intrinsics user_intrinsics L0_trace in
+  let L1_trace        := build_L1 L0_trace' in
+  let L2_trace        := build_L2 L1_trace in
+  let L3_trace        := build_L3 L2_trace in
+  L3_trace.
+
+Definition build_to_L4 (user_intrinsics: IS.intrinsic_definitions) (prog: mcfg typ) :=
+  let mcfg := normalize_types prog in
+
+  let L0_trace        := build_L0 mcfg in
+  let L0_trace'       := INT.interpret_intrinsics user_intrinsics L0_trace in
+  let L1_trace        := build_L1 L0_trace' in
+  let L2_trace        := build_L2 L1_trace in
+  let L3_trace        := build_L3 L2_trace in
+  let L4_trace        := model_L4 L3_trace in
+  L4_trace.
+
+Definition refine_mcfg_L1 (p1 p2: mcfg typ): Prop :=
+  R.refine_L1 (build_to_L1 nil p1) (build_to_L1 nil p2).
+
+Definition refine_mcfg_L2 (p1 p2: mcfg typ): Prop :=
+  R.refine_L2 (build_to_L2 nil p1) (build_to_L2 nil p2).
+
+Definition refine_mcfg_L3 (p1 p2: mcfg typ): Prop :=
+  R.refine_L3 (build_to_L3 nil p1) (build_to_L3 nil p2).
+
+Definition refine_mcfg_L4 (p1 p2: mcfg typ): Prop :=
+  R.refine_L4 (build_to_L4 nil p1) (build_to_L4 nil p2).
+
+Definition refine_mcfg (p1 p2: mcfg typ): Prop :=
+  R.refine_L5 (model_mcfg p1) (model_mcfg p2).
+
+Lemma refine_mcfg_L1_correct: forall p1 p2,
+    refine_mcfg_L1 p1 p2 -> refine_mcfg p1 p2.
+Admitted.
+
+Lemma refine_mcfg_L2_correct: forall p1 p2,
+    refine_mcfg_L2 p1 p2 -> refine_mcfg p1 p2.
+Proof.
+Admitted.
+
+Lemma refine_mcfg_L3_correct: forall p1 p2,
+    refine_mcfg_L3 p1 p2 -> refine_mcfg p1 p2.
+Proof.
+Admitted.
+
+Lemma refine_mcfg_L4_correct: forall p1 p2,
+    refine_mcfg_L4 p1 p2 -> refine_mcfg p1 p2.
+Proof.
+Admitted.
+
+
+(* TODO SCRAPYARD, TO RECYCLE OR BURN
 Instance refine_uvalue_refl :
   Reflexive refine_uvalue.
 Proof.
@@ -112,39 +240,7 @@ Proof.
   apply Reflexive_eqit.
   repeat apply prod_rel_refl; auto using TT_refl, refine_uvalue_refl.
 Qed.
-
-Instance interp_prop_Proper :
-  forall R E F G (t : itree (E +' G) R) (RR : relation R) (h : (E +' F +' G) ~> PropT.PropT (itree (E +' G))),
-    Proper (@eutt (E +' F +' G) _ _ RR ==> iff) (fun t' => @PropT.interp_prop (E +' F +' G) _ _ _ _ h _ t' t).
-Proof.
-  intros R E F G t RR h.
-  intros t1 t2 Heutt.
-  unfold PropT.PropT in h. unfold Ensembles.Ensemble in h.
-Admitted.
-
-Lemma refine_34 : forall t1 t2,
-    refine_L3 t1 t2 -> refine_L4 (model_L4 t1) (model_L4 t2).
-Proof.
-  intros t1 t2 H.
-  unfold refine_L4.
-  intros t Hip.
-
-  unfold model_L4 in *.
-  unfold P.model_undef in *.
-
-  exists t; split.
-
-  match goal with
-  | [ |- context [PropT.interp_prop ?h _ _] ] =>
-    apply (interp_prop_Proper res_L3 _ _ _ t refine_res3 h t1 t2 H)
-  end.
-
-  apply Hip.
-
-  apply Reflexive_eqit.
-  repeat apply prod_rel_refl; auto using TT_refl, refine_uvalue_refl.
-Qed.
-
+*)
 
 (* Unfinished proof *)
 (*
@@ -161,7 +257,7 @@ Proof.
   intros x0 x1 PR.
   unfold refine_res4.
   eapply subrelation_prod_left. apply subrelation_R_TT with (R:=eq). apply PR.
-  
+
 Qed.
  *)
 
@@ -191,3 +287,4 @@ Proof.
   repeat apply prod_rel_refl; auto using TT_refl, refine_uvalue_refl.
 Qed.
  *)
+
